Added patition left and right

theories/quicksort.v
@@ -1,4 +1,139 @@
+
 Set Warnings "-notation-overridden,-parsing,-deprecated-hint-without-locality".
-From Quicksort Require Import arraylist.
-From Quicksort Require Import shuffle.
+From Coq Require Export Bool.Bool.
+From Coq Require Export Arith.Arith.
+From Coq Require Export Arith.EqNat.
+From Coq Require Export Lia.
+From Coq Require Export Lists.List.
+Export ListNotations.
+From Coq Require Export Permutation.
+From Coq Require Export Numbers.NatInt.NZDiv.
+
+(*Arraylist code*)
+Fixpoint lookup (i : nat) (l : list nat) := 
+    match l with
+    | [] => 0
+    | h :: t => if i <=? 0 then h else lookup (i-1) t
+    end.
+   
+
+Example lookup_example1 :
+    lookup 3 [2;3;4;5;1;2] = 5.
+Proof. simpl. reflexivity. Qed.
+
+Example lookup_example_empty_list :
+    lookup 3 [] = 0.
+Proof. simpl. reflexivity. Qed.
+
+Example lookup_example_higher_than_list :
+    lookup 10 [2;3;4;5;1;2] = 0.
+Proof. simpl. reflexivity. Qed.
+
+
+Fixpoint insert (elem : nat) (index : nat) (l : list nat) :=
+match (index, l) with
+| (0, x::xs) => elem :: xs
+| (0, []) => [elem] (* should never happen *)
+| (n, x::xs) => x :: (insert elem (index-1) xs)
+| (n, []) => [elem] (* should never happen *)
+end.
+
+Example insert_example1:
+    insert 3 1 [2;2;2] = [2;3;2].
+Proof.
+    trivial.
+Qed.
+
+Example insert_example2:
+    insert 3 0 [2] = [3].
+Proof.
+    trivial.
+Qed.
+
+(*Shuffle code*)
+
+Definition randnat (seed : nat) (bound : nat) : nat :=
+    (seed*31+7) mod bound.
+
+Definition fst3 (tuple : (list nat*nat*nat)) : list nat :=
+    match tuple with
+    | (a,b,c) => a
+    end.
+
+Definition swap (l : list nat) (i1 : nat) (i2 : nat) : list nat :=
+    insert (lookup i2 l) i1 (insert (lookup i1 l) i2 l).
+
+Example swap_example1:
+    swap [1;2;3;4] 0 3 = [4;2;3;1].
+Proof.
+    trivial.
+Qed.
+
+Example swap_example2:
+    swap [1;2;3;4;5] 0 3 = [4;2;3;1;5].
+Proof.
+    trivial.
+Qed.
+
+Definition shuffle (l : list nat) : list nat :=
+    fst3 (List.fold_left (fun (acc : ((list nat)*nat*nat)) (a : nat) =>
+            match acc with
+            | (li,seed,point) => (swap li point (randnat seed (List.length li)) ,seed+1,point+1)
+            end) l (l,42,0)).
+
+Example shuffle_example1:
+    shuffle [1;2;3;4;5] = [2;3;4;1;5]. (*pseudorandom order*)
+Proof.
+    reflexivity.
+Qed.
+
+
+(*Quicksort code*)
+Fixpoint partition_left (l : list nat) (pivot : nat) (lo : nat) (hi : nat) : nat :=
+    if ((lookup l lo < pivot) && (lo < hi)) then partition_left l pivot (lo+1) else lo
+.    
+
+
+Fixpoint partition_right (l : list nat) (pivot : nat) (lo : nat) (hi : nat) : nat :=
+    if ((lookup l hi > pivot) && (lo < hi)) then partition_right l pivot (hi-1) else hi
+    
+
+
+
+
+Fixpoint partition2 (l : list nat) (pivot : nat) (lo : nat) (hi : nat) : list nat :=
+    (*
+    match (lo,hi) with
+    | ((lookup hi l > pivot) && (lookup lo l < pivot)) => partition2 l pivot (lo+1) (hi-1)
+    | ((lookup hi l > pivot) && (lookup lo l > pivot)) => partition2 l pivot (lo) (hi-1)
+    | ((lookup hi l < pivot) && (lookup lo l < pivot)) => partition2 l pivot (lo+1) (hi)
+    | ((lookup hi l < pivot) && (lookup lo l > pivot)) => partition2 (swap l lo hi) pivot (lo+1) (hi-1)
+    *)
+
+
+    match ((partition_left l pivot lo hi), (partition_right l pivot lo hi)) with
+    | (lo, hi) => if lo < hi then partition2 (swap l lo hi) pivot (lo+1) (hi-1) else l
+
+    end
+
+
+
+
+
+
+
+(* Fixpoint partition (l : list nat) (lo : nat) (hi : nat) : list nat :=
+    match l with
+    | [] => l
+    | [x] => l 
+    | [h :: t] => 
+
+
+
+
+
+Definition quicksort (l : list nat) : list nat :=
+    shuffle l *)
+
+
 
